finish getting holSemanticsTheory to build again
the rest of the implementation (hol_{kernel,verification} and
ml_hol_kernel) still needs updating.

hol-light/holSemanticsScript.sml
@@ -1184,24 +1184,6 @@ val TERM_UNION_FILTER_NIL = store_thm("TERM_UNION_FILTER_NIL",
   METIS_TAC[])
 val _ = export_rewrites["TERM_UNION_FILTER_NIL"]
 
-val def_ok_def = Define`
-  (def_ok (Constdef eqs p) ⇔
-    EVERY (λt. CLOSED t ∧ set (tvars t) ⊆ set (tyvars (typeof t)))
-     (MAP SND eqs)) ∧
-  (def_ok (Typedef n t a r) ⇔ ∃rty. CLOSED t ∧ t has_type Fun rty Bool)`
-
-val deftm_def = Define`
-  deftm (Constdef eqs p) = MAP SND eqs ++ MAP (λ(s,t).Const s (typeof t)) eqs ∧
-  deftm (Typedef n t a r) =
-  let rty = domain(typeof t) in
-  let aty = Tyapp n (MAP Tyvar (STRING_SORT (tvars t))) in
-    [t;Const a (Fun rty aty);Const r (Fun aty rty)]`
-
-val defcnds_ok_def = Define`
-  (defcnds_ok [] ⇔ T) ∧
-  (defcnds_ok ((Typedef _ t _ _)::defs) ⇔ (∃w. (defs,[]) |- Comb t w) ∧ defcnds_ok defs) ∧
-  (defcnds_ok ((Constdef eqs p)::defs) ⇔ term_ok defs p ∧ EVERY (term_ok defs) (MAP SND eqs) ∧ defcnds_ok defs)`
-
 fun memdef n =
   last(CONJUNCTS holSyntaxTheory.proves_rules)
   |> SPEC_ALL |> concl |> dest_imp |> fst |> strip_conj
@@ -1353,6 +1335,34 @@ val term_Forall = store_thm("term_Forall",
   simp[holSyntaxTheory.EQUATION_HAS_TYPE_BOOL,welltyped_equation] >>
   simp[equation_def,holSyntaxTheory.equation_def])
 
+val def_ok_def = Define`
+  (def_ok (Constdef eqs p) ⇔
+    EVERY (λt. CLOSED t ∧ set (tvars t) ⊆ set (tyvars (typeof t)))
+     (MAP SND eqs) ∧
+    ALL_DISTINCT (MAP FST eqs) ∧
+    (∀x ty. VFREE_IN (Var x ty) p ⇒ ∃t. MEM (x,t) eqs ∧ typeof t = ty)) ∧
+  (def_ok (Typedef n t a r) ⇔ ∃rty. CLOSED t ∧ t has_type Fun rty Bool)`
+
+val deftm_def = Define`
+  deftm (Constdef eqs p) =
+    p::MAP SND eqs ++
+    MAP (λ(s,t).Const s (typeof t)) eqs ∧
+  deftm (Typedef n t a r) =
+  let rty = domain(typeof t) in
+  let aty = Tyapp n (MAP Tyvar (STRING_SORT (tvars t))) in
+    [t;Const a (Fun rty aty);Const r (Fun aty rty)]`
+
+val defcnds_ok_def = Define`
+  (defcnds_ok [] ⇔ T) ∧
+  (defcnds_ok ((Typedef _ t _ _)::defs) ⇔ (∃w. (defs,[]) |- Comb t w) ∧ defcnds_ok defs) ∧
+  (defcnds_ok ((Constdef eqs p)::defs) ⇔
+    (defs, MAP (λ(s,t). Var s (typeof t) === t) eqs) |- p (* ∧
+    term_ok defs p ∧ EVERY (term_ok defs) (MAP SND eqs)*) ∧ defcnds_ok defs)`
+
+val defthm_def = Define`
+  defthm (Constdef eqs p) = [(MAP (λ(s,t). Var s (typeof t) === t) eqs, p)] ∧
+  defthm _ = []`
+
 val proves_IMP = store_thm("proves_IMP",
   ``is_model M ⇒
     (∀defs ty. type_ok defs ty ⇒ context_ok defs ∧ good_defs defs ∧ ∃ty1. type defs ty ty1 ∧ type_ok ty1) ∧
@@ -1361,13 +1371,15 @@ val proves_IMP = store_thm("proves_IMP",
       good_defs defs ∧
       EVERY def_ok defs ∧
       defcnds_ok defs ∧
-      (∀t. MEM t (FLAT (MAP deftm defs)) ⇒ term_ok defs t ∧ ∃t1. term defs t t1 ∧ term_ok t1)) ∧
+      (∀t. MEM t (FLAT (MAP deftm defs)) ⇒ term_ok defs t ∧ ∃t1. term defs t t1 ∧ term_ok t1) ∧
+      (∀h c. MEM (h,c) (FLAT (MAP defthm defs)) ⇒ ∃h1 c1. seq_trans ((defs,h),c) (h1,c1) ∧ h1 |- c1)) ∧
     (∀dh c. dh |- c ⇒
       context_ok (FST dh) ∧
       good_defs (FST dh) ∧
       EVERY def_ok (FST dh) ∧
       defcnds_ok (FST dh) ∧
       (∀t. MEM t (FLAT (MAP deftm (FST dh))) ⇒ term_ok (FST dh) t ∧ ∃t1. term (FST dh) t t1 ∧ term_ok t1) ∧
+      (∀h c. MEM (h,c) (FLAT (MAP defthm (FST dh))) ⇒ ∃h1 c1. seq_trans ((FST dh,h),c) (h1,c1) ∧ h1 |- c1) ∧
       ∃h1 c1. seq_trans (dh,c) (h1,c1) ∧ h1 |- c1)``,
   strip_tac >>
   HO_MATCH_MP_TAC holSyntaxTheory.proves_strongind >>
@@ -1762,7 +1774,9 @@ val proves_IMP = store_thm("proves_IMP",
       simp[MAP_MAP_o,combinTheory.o_DEF,UNCURRY,ETA_AX] >>
       METIS_TAC[] ) >>
     conj_asm1_tac >- (
-      simp[def_ok_def,pred_setTheory.SUBSET_DEF] ) >>
+      simp[def_ok_def,pred_setTheory.SUBSET_DEF] >>
+      fs[ALL_DISTINCT_APPEND,MEM_MAP,EXISTS_PROD] >>
+      METIS_TAC[]) >>
     `∀t. MEM t (MAP SND eqs) ⇒ term_ok defs t` by (
       simp[MEM_MAP,EXISTS_PROD,GSYM LEFT_FORALL_IMP_THM] >>
       qx_genl_tac[`t`,`s`] >> strip_tac >>
@@ -1777,14 +1791,15 @@ val proves_IMP = store_thm("proves_IMP",
       map_every qexists_tac[`hh`,`cc`] >>
       simp[Abbr`hh`,MEM_MAP,EXISTS_PROD] >>
       METIS_TAC[] ) >>
-    conj_asm1_tac >- (
-      simp[defcnds_ok_def] >>
+    conj_asm1_tac >- simp[defcnds_ok_def] >>
+    (*
       conj_tac >- (
         simp[Once holSyntaxTheory.proves_cases] >>
         METIS_TAC[] ) >>
       simp[EVERY_MEM,EVERY_MAP,FORALL_PROD] >>
       fs[MEM_MAP,EXISTS_PROD,GSYM LEFT_FORALL_IMP_THM] >>
       METIS_TAC[] ) >>
+    *)
     simp[DISJ_IMP_THM] >>
     simp[FORALL_AND_THM] >>
     simp[GSYM CONJ_ASSOC] >>
@@ -1819,6 +1834,18 @@ val proves_IMP = store_thm("proves_IMP",
           simp[Once proves_cases,MEM_EL] >>
           METIS_TAC[]) >>
         METIS_TAC[soundness,has_meaning_welltyped] ) >>
+    `term_ok defs c'` by (
+      simp[Once holSyntaxTheory.proves_cases] >>
+      METIS_TAC[] ) >>
+    conj_asm1_tac >- (
+      first_x_assum match_mp_tac >>
+      simp[] ) >>
+    conj_asm1_tac >- (
+      res_tac >>
+      qexists_tac`c1'` >>
+      simp[] >>
+      simp[Once proves_cases] >>
+      METIS_TAC[] ) >>
     conj_asm1_tac >- (
       ntac 2 strip_tac >> simp[] >>
       pop_assum mp_tac >>
@@ -1960,61 +1987,204 @@ val proves_IMP = store_thm("proves_IMP",
       last_x_assum(qspec_then`t`mp_tac) >>
       simp[PULL_EXISTS] >>
       METIS_TAC[] ) >>
+    simp[defthm_def] >>
+    conj_tac >- (
+      qexists_tac`h1'` >>
+      qexists_tac`c1'` >>
+      simp[] >>
+      BasicProvers.VAR_EQ_TAC >>
+      simp[EVERY2_EVERY,GSYM AND_IMP_INTRO,EVERY_MEM,MEM_ZIP,PULL_EXISTS,EL_MAP,UNCURRY] >>
+      rw[] >>
+      match_mp_tac term_equation_matchable >>
+      simp[holSyntaxTheory.EQUATION_HAS_TYPE_BOOL] >>
+      first_x_assum(qspec_then`n`mp_tac) >>
+      simp[holSyntaxTheory.WELLTYPED] >>
+      strip_tac >>
+      imp_res_tac has_type_IMP >>
+      imp_res_tac WELLTYPED_LEMMA >>
+      rw[] >>
+      qunabbrev_tac`ddefs` >>
+      match_mp_tac(MP_CANON (CONJUNCT1 (UNDISCH (SPEC_ALL term_type_cons)))) >>
+      simp[safe_def_names_def,pred_setTheory.IN_DISJOINT] >>
+      fs[ALL_DISTINCT_APPEND,MEM_MAP] >>
+      METIS_TAC[]) >>
+    conj_tac >- (
+      rw[] >>
+      res_tac >>
+      qexists_tac`h1'` >>
+      fs[EVERY2_EVERY,GSYM AND_IMP_INTRO,EVERY_MEM,MEM_ZIP,PULL_EXISTS] >>
+      rfs[EVERY2_EVERY,GSYM AND_IMP_INTRO,EVERY_MEM,MEM_ZIP,PULL_EXISTS] >>
+      METIS_TAC[] ) >>
     qpat_assum`LIST_REL X Y h1`mp_tac >>
     simp[EVERY2_EVERY,GSYM AND_IMP_INTRO,EVERY_MEM,MEM_ZIP,PULL_EXISTS] >>
     ntac 2 strip_tac >>
     qexists_tac`h1` >>
     simp[MEM_ZIP,PULL_EXISTS] >>
     qexists_tac`c1` >> simp[]) >>
-
   conj_tac >- (
     rw[seq_trans_def] >>
-    first_x_assum(qspec_then`t`mp_tac) >>
-    simp[MEM_FLAT,MEM_MAP] >>
+    Q.PAT_ABBREV_TAC`ilist:(holSyntax$term#holSyntax$term)list = MAP X eqs` >>
+    first_x_assum(qspecl_then[`MAP (λ(s,t). Var s (typeof t) === t) eqs`,`p`]mp_tac) >>
     discharge_hyps >- (
-      srw_tac[boolSimps.DNF_ss][] >>
-      qexists_tac`Constdef n t` >>
-      simp[deftm_def] ) >>
-    strip_tac >>
-    `welltyped t1` by (
-      imp_res_tac soundness >>
-      METIS_TAC[has_meaning_welltyped] ) >>
-    `welltyped t` by METIS_TAC[term_welltyped] >>
-    qexists_tac`Const n (typeof t1) (Defined t1) === t1` >>
-    qspecl_then[`Const n (typeof t)`,`t`]mp_tac term_equation >>
-    simp[holSyntaxTheory.EQUATION_HAS_TYPE_BOOL] >> strip_tac >>
+      simp[MEM_MAP,MEM_FLAT,PULL_EXISTS] >>
+      qexists_tac`Constdef eqs p` >>
+      simp[defthm_def] ) >>
+    disch_then(qx_choosel_then[`eqs1`,`p1`]strip_assume_tac) >>
+    `∃vs1. LIST_REL (λ(x,t) e. e = Var x (typeof t) === t ∧ welltyped e) vs1 eqs1` by (
+      simp[EVERY2_EVERY,EVERY_MEM,exists_list_GENLIST,MEM_ZIP,PULL_EXISTS,UNCURRY,GSYM SKOLEM_THM] >>
+      fs[EVERY2_EVERY,EVERY_MEM] >> rfs[MEM_ZIP,PULL_EXISTS,EL_MAP,UNCURRY] >>
+      rw[RIGHT_EXISTS_IMP_THM] >>
+      res_tac >>
+      qmatch_assum_abbrev_tac`term defs (e1 === e2) e` >>
+      qspecl_then[`e1`,`e2`,`e`]mp_tac term_equation >>
+      `welltyped e` by (
+        imp_res_tac soundness >>
+        fs[sequent_def,EVERY_MEM] >>
+        METIS_TAC[MEM_EL,has_meaning_welltyped] ) >>
+      imp_res_tac term_welltyped >>
+      fs[welltyped_equation] >> rw[Abbr`e`] >>
+      simp[Abbr`e1`] >> fs[EXISTS_PROD] >>
+      fs[holSyntaxTheory.EQUATION_HAS_TYPE_BOOL] >>
+      fs[holSyntaxTheory.WELLTYPED] >>
+      imp_res_tac has_type_IMP >>
+      imp_res_tac term_type_11 >>
+      rw[] >>
+      METIS_TAC[WELLTYPED_LEMMA]) >>
+    qexists_tac`VSUBST (GENLIST
+      (λn. let x = FST(EL n eqs) in
+           let ty = typeof(SND(EL n vs1)) in
+      (Const x ty (Defined n vs1 p1),
+       Var x ty)) (LENGTH eqs)) p1` >>
     conj_tac >- (
-      qexists_tac`Const n (typeof t1) (Defined t1)` >>
-      qexists_tac`t1` >>
+      match_mp_tac VSUBST_IMP >>
+      simp[MAP_GENLIST,combinTheory.o_DEF] >>
+      simp[EVERY2_EVERY,EVERY_MEM,GSYM AND_IMP_INTRO,MEM_ZIP
+          ,Abbr`ilist`,PULL_EXISTS,EL_MAP,MEM_MAP] >>
+      simp[UNCURRY,MEM_GENLIST,PULL_EXISTS] >>
+      simp[Once has_type_cases] >>
+      simp[Once holSyntaxTheory.has_type_cases] >>
+      reverse conj_asm2_tac >- (
+        fs[EVERY2_EVERY,EVERY_MEM] >>
+        rfs[MEM_ZIP,PULL_EXISTS,EL_MAP,UNCURRY] >>
+        rw[] >> res_tac >>
+        imp_res_tac term_welltyped >>
+        fs[welltyped_equation] >>
+        qmatch_assum_abbrev_tac`term defs (e1 === e2) e` >>
+        qspecl_then[`e1`,`e2`,`e`]mp_tac term_equation >>
+        simp[] >> simp[Abbr`e1`,Abbr`e2`]) >>
+      rw[] >>
+      match_mp_tac(List.nth(CONJUNCTS (SPEC_ALL term_rules),10)) >>
+      qexists_tac`eqs` >> qexists_tac`p` >>
       simp[] >>
-      simp[Once term_cases] >>
-      imp_res_tac MEM_Constdef_const_def >>
-      qexists_tac`t` >>
-      simp[] >>
-      METIS_TAC[good_defs_def,has_type_IMP,WELLTYPED_LEMMA,WELLTYPED,holSyntaxTheory.WELLTYPED_LEMMA,holSyntaxTheory.WELLTYPED]) >>
+      conj_tac >- (
+        match_mp_tac MEM_Constdef_const_def >>
+        fs[good_defs_def] >>
+        Q.ISPECL_THEN[`MAP FST eqs`,`n`,`0:num`]mp_tac find_index_ALL_DISTINCT_EL >>
+        discharge_hyps >- (
+          simp[] >> fs[EVERY_MEM] >>
+          res_tac >> fs[def_ok_def] ) >>
+        simp[EL_MAP] ) >>
+      fs[EVERY2_EVERY,EVERY_MEM] >>
+      rfs[MEM_ZIP,PULL_EXISTS,EL_MAP,UNCURRY] >>
+      simp[Once LIST_EQ_REWRITE,EL_MAP,GSYM FORALL_AND_THM,GSYM IMP_CONJ_THM] >>
+      qx_gen_tac`m`>>strip_tac >>
+      rpt(first_x_assum(qspec_then`m`mp_tac)) >>
+      simp[] >> ntac 3 strip_tac >>
+      qmatch_assum_abbrev_tac`term defs (e1 === e2) e` >>
+      qspecl_then[`e1`,`e2`,`e`]mp_tac term_equation >>
+      discharge_hyps >- (
+        imp_res_tac term_welltyped >> fs[welltyped_equation] ) >>
+      simp[Abbr`e1`] ) >>
     match_mp_tac(List.nth(CONJUNCTS proves_rules,25)) >>
-    fs[WELLTYPED] >>
-    fs[EVERY_MEM] >>
-    res_tac >> fs[def_ok_def] >>
-    imp_res_tac CLOSED_IMP >> simp[] >>
-    imp_res_tac tvars_IMP >>
-    fs[holSyntaxTheory.WELLTYPED] >>
-    imp_res_tac has_type_IMP >>
-    imp_res_tac tyvars_IMP >>
-    imp_res_tac WELLTYPED_LEMMA >>
-    METIS_TAC[]) >>
+    simp[] >>
+    qexists_tac`vs1` >>
+    `eqs1 = MAP (λ(s,t). Var s (typeof t) === t) vs1` by (
+      fs[EVERY2_EVERY,EVERY_MEM] >>
+      rfs[MEM_ZIP,PULL_EXISTS,UNCURRY] >>
+      simp[Once LIST_EQ_REWRITE,EL_MAP,UNCURRY] ) >>
+    conj_tac >- rw[] >>
+    `MAP FST eqs = MAP FST vs1 ∧ LIST_REL (term defs) (MAP SND eqs) (MAP SND vs1)` by (
+      fs[EVERY2_EVERY,EVERY_MEM] >>
+      simp[Once LIST_EQ_REWRITE,EL_MAP] >>
+      rfs[MEM_ZIP,UNCURRY,PULL_EXISTS,EL_MAP] >>
+      simp[GSYM FORALL_AND_THM,GSYM IMP_CONJ_THM] >>
+      ntac 2 strip_tac >>
+      res_tac >>
+      qmatch_assum_abbrev_tac`term defs (e1 === e2) e` >>
+      qspecl_then[`e1`,`e2`,`e`]mp_tac term_equation >>
+      discharge_hyps >- (
+        imp_res_tac term_welltyped >> fs[welltyped_equation] ) >>
+      simp[Abbr`e1`,Abbr`e`] ) >>
+    `def_ok (Constdef eqs p)` by METIS_TAC[EVERY_MEM] >>
+    fs[def_ok_def] >>
+    conj_tac >- (
+      fs[EVERY_MAP,EVERY2_EVERY,EVERY_MEM] >>
+      rfs[MEM_ZIP,PULL_EXISTS,MEM_EL,EL_MAP] >>
+      qx_gen_tac`m`>>strip_tac >> res_tac >>
+      imp_res_tac CLOSED_IMP >>
+      imp_res_tac tvars_IMP >>
+      fs[UNCURRY] >>
+      qpat_assum`welltyped X`mp_tac >>
+      simp_tac(srw_ss())[Once WELLTYPED] >>
+      simp[Once equation_def,SimpR``$has_type``,EQUATION_HAS_TYPE_BOOL] >>
+      strip_tac >>
+      imp_res_tac term_welltyped >>
+      fs[holSyntaxTheory.WELLTYPED] >>
+      imp_res_tac has_type_IMP >>
+      imp_res_tac WELLTYPED_LEMMA >>
+      imp_res_tac tyvars_IMP >>
+      fs[] ) >>
+    conj_tac >- (
+      match_mp_tac (Q.ISPEC`FST`ALL_DISTINCT_MAP) >>
+      simp[MAP_MAP_o,combinTheory.o_DEF,UNCURRY,ETA_AX] >>
+      METIS_TAC[] ) >>
+    conj_tac >- (
+      rw[] >>
+      qspecl_then[`p1`,`defs`,`p`,`Var x ty`]mp_tac term_subterm_inv >>
+      simp[PULL_EXISTS] >>
+      Cases >> TRY(simp[Once term_cases]>>NO_TAC) >>
+      simp[MEM_MAP,EXISTS_PROD] >>
+      fs[EVERY2_EVERY,EVERY_MEM] >>
+      rw[] >> res_tac >>
+      rfs[MEM_ZIP,MEM_EL,PULL_EXISTS,EL_MAP] >>
+      rpt(first_x_assum(qspec_then`n`mp_tac)) >>
+      rw[UNCURRY] >>
+      CONV_TAC SWAP_EXISTS_CONV >>
+      qexists_tac`n` >> simp[] >>
+      Cases_on`EL n vs1`>>fs[] >>
+      qpat_assum`MAP X Y = MAP A B`mp_tac >>
+      simp[Once LIST_EQ_REWRITE,EL_MAP] >>
+      disch_then(qspec_then`n`mp_tac) >> simp[] >>
+      qpat_assum`X = EL n eqs`(assume_tac o SYM) >> simp[] >>
+      fs[] >>
+      qpat_assum`welltyped X`mp_tac >>
+      simp_tac(srw_ss())[Once WELLTYPED] >>
+      simp[Once equation_def,SimpR``$has_type``,EQUATION_HAS_TYPE_BOOL] >>
+      strip_tac >>
+      imp_res_tac term_welltyped >>
+      fs[holSyntaxTheory.WELLTYPED] >>
+      imp_res_tac has_type_IMP >>
+      imp_res_tac WELLTYPED_LEMMA >>
+      fs[] >>
+      imp_res_tac term_type_11 >>
+      rw[]) >>
+    simp[LIST_EQ_REWRITE] >>
+    conj_asm1_tac >- fs[EVERY2_EVERY] >>
+    simp[EL_GENLIST,EL_MAP,UNCURRY] >>
+    qpat_assum`MAP FST X = MAP FST Y`mp_tac >>
+    simp[Once LIST_EQ_REWRITE,EL_MAP] ) >>
   conj_tac >- (
     rpt gen_tac >>
     simp[seq_trans_def] >>
     simp[GSYM AND_IMP_INTRO] >>
-    ntac 15 strip_tac >>
+    ntac 16 strip_tac >>
     rpt BasicProvers.VAR_EQ_TAC >>
     qmatch_abbrev_tac`P ⇒ A ∧ B ∧ C` >>
     `A` by (
       simp[Abbr`A`] >>
       simp[Once holSyntaxTheory.proves_cases] >>
       map_every qexists_tac[`[]`,`holSyntax$Comb t y`] >>
-      match_mp_tac (List.nth(CONJUNCTS holSyntaxTheory.proves_rules,25)) >>
+      match_mp_tac (List.nth(CONJUNCTS holSyntaxTheory.proves_rules,26)) >>
       simp[] >>
       map_every qexists_tac[`rep_type`,`y`] >>
       METIS_TAC[] ) >>
@@ -2045,16 +2215,26 @@ val proves_IMP = store_thm("proves_IMP",
       rpt gen_tac >>
       simp(List.map Abbr [`B`,`C`,`P`,`Q`,`R`]) >>
       strip_tac >>
-      map_every qexists_tac[`h1`,`c1'`] >>
-      fs[EVERY_MEM,EVERY2_EVERY] >>
-      rfs[MEM_ZIP,GSYM LEFT_FORALL_IMP_THM] >>
+      simp[defthm_def] >>
       `safe_def_names defs (Typedef tyname t a r)` by (
         simp[safe_def_names_def] ) >>
+      rw[] >> res_tac >|[map_every qexists_tac[`h1'`,`c1''`],
+                         map_every qexists_tac[`h1`,`c1'`]] >>
+      fs[EVERY_MEM,EVERY2_EVERY] >>
+      rfs[MEM_ZIP,GSYM LEFT_FORALL_IMP_THM] >>
       METIS_TAC[term_type_cons]) >>
     `∀asl c. Q asl c ⇒ C asl c` by (
       rpt gen_tac >>
       simp(List.map Abbr [`B`,`C`,`P`,`Q`,`R`]) >>
-      rw[] >>
+      simp[defthm_def] >>
+      rw[] >- (
+        `safe_def_names defs (Typedef tyname t a r)` by (
+          simp[safe_def_names_def] ) >>
+        res_tac >>
+        map_every qexists_tac[`h1`,`c1'`] >>
+        fs[EVERY_MEM,EVERY2_EVERY] >>
+        rfs[MEM_ZIP,GSYM LEFT_FORALL_IMP_THM] >>
+        METIS_TAC[term_type_cons]) >>
       qho_match_abbrev_tac`∃e1. term ddefs (t1 === t2) e1 ∧ [] |- e1` >>
       rfs[] >>
       qmatch_assum_abbrev_tac`Abbrev (t2 = Var x ty)` >>
@@ -2069,8 +2249,6 @@ val proves_IMP = store_thm("proves_IMP",
       simp[Abbr`t2`] >>
       simp_tac(srw_ss()++boolSimps.DNF_ss)[] >>
       simp[Once CONJ_COMM] >>
-      simp[Once term_cases] >>
-      simp_tac(srw_ss()++boolSimps.DNF_ss)[] >>
       simp[Abbr`ty`] >>
       simp[Once term_cases] >>
       simp_tac(srw_ss()++boolSimps.DNF_ss)[] >>
@@ -2104,55 +2282,54 @@ val proves_IMP = store_thm("proves_IMP",
       simp[Once const_def_def] >>
       simp[Once type_def_def] >>
       simp[Once const_def_def] >>
-      simp[Once term_cases] >>
-      simp_tac(srw_ss()++boolSimps.DNF_ss)[] >>
       `∃ty1. x1 has_type ty1 ∧ type defs (Fun rep_type Bool) ty1` by METIS_TAC[has_type_IMP] >>
-      pop_assum mp_tac >>
-      simp[Once term_cases] >>
-      simp_tac(srw_ss()++boolSimps.DNF_ss)[] >>
-      rpt strip_tac >>
-      pop_assum mp_tac >>
-      simp[Once term_cases] >>
-      strip_tac >>
-      rpt BasicProvers.VAR_EQ_TAC >>
+      pop_assum mp_tac >> simp[] >>
+      disch_then(qx_choose_then`r1`strip_assume_tac) >>
       CONV_TAC SWAP_EXISTS_CONV >>
       qexists_tac`x1` >>
       CONV_TAC SWAP_EXISTS_CONV >>
-      qexists_tac`tx1` >>
-      simp[Q.SPEC`Comb X Y`(CONJUNCT2 (SPEC_ALL term_cases))] >>
+      qexists_tac`r1` >>
+      `type (Typedef tyname t a r::defs) rep_type r1` by (
+        match_mp_tac (MP_CANON(CONJUNCT1 (UNDISCH(SPEC_ALL term_type_cons)))) >>
+        simp[safe_def_names_def] ) >>
+      simp[] >>
+      simp[Once term_cases] >>
       simp_tac(srw_ss()++boolSimps.DNF_ss)[] >>
-      simp[Q.SPEC`Var X Y`(CONJUNCT2 (SPEC_ALL term_cases))] >>
+      simp[Once type_def_def] >>
+      CONV_TAC SWAP_EXISTS_CONV >>
+      qexists_tac`x1` >> simp[] >>
+      CONV_TAC SWAP_EXISTS_CONV >>
+      HINT_EXISTS_TAC >> simp[] >>
+      simp[Once term_cases] >>
       simp_tac(srw_ss()++boolSimps.DNF_ss)[] >>
+      simp[Once(CONJUNCT1 (SPEC_ALL term_cases))] >>
+      simp_tac(srw_ss()++boolSimps.DNF_ss)[] >>
+      simp[Once type_def_def] >>
+      CONV_TAC SWAP_EXISTS_CONV >>
+      qexists_tac`x1` >> simp[] >>
+      CONV_TAC SWAP_EXISTS_CONV >>
+      HINT_EXISTS_TAC >> simp[] >>
       simp[Q.SPEC`Const X Y`(CONJUNCT2 (SPEC_ALL term_cases))] >>
       simp[Once const_def_def] >>
       simp[Once const_def_def] >>
       simp_tac(srw_ss()++boolSimps.DNF_ss)[] >>
       `r ≠ "="` by fs[consts_def] >> simp[] >>
-      simp[Q.SPEC`Fun X Y`(CONJUNCT1 (SPEC_ALL term_cases))] >>
-      simp_tac(srw_ss()++boolSimps.DNF_ss)[] >>
       simp[Q.SPEC`Tyapp X Y`(CONJUNCT1 (SPEC_ALL term_cases))] >>
       simp_tac(srw_ss()++boolSimps.DNF_ss)[] >>
       simp[Once type_def_def] >>
       simp[Once type_def_def] >>
-      simp[Once type_def_def] >>
       simp[Once const_def_def] >>
       `safe_def_names defs (Typedef tyname t a r)` by simp[safe_def_names_def] >>
-      `type (Typedef tyname t a r::defs) rep_type tx1` by METIS_TAC[term_type_cons] >>
       qexists_tac`x1` >> simp[] >>
-      qexists_tac`tx1` >> simp[] >>
+      qexists_tac`r1` >> simp[] >>
       qexists_tac`x1` >> simp[] >>
       qmatch_assum_abbrev_tac`LIST_REL ff ll rr` >>
-      qexists_tac`rr` >> simp[] >>
-      qexists_tac`x1` >> simp[] >>
-      qexists_tac`rr` >> simp[] >>
-      simp[Once type_def_def] >>
-      qexists_tac`x1` >> simp[] >>
       qexists_tac`rr` >> simp[] >>
       reverse conj_tac >- (
         rw[] >>
         imp_res_tac MEM_Typedef_MEM_consts >>
         fs[consts_def]) >>
-      match_mp_tac(List.nth(CONJUNCTS proves_rules,26)) >>
+      match_mp_tac(List.nth(CONJUNCTS proves_rules,27)) >>
       imp_res_tac CLOSED_IMP >>
       simp[] >>
       qexists_tac`y1` >>
@@ -2161,13 +2338,22 @@ val proves_IMP = store_thm("proves_IMP",
       `welltyped x1` by METIS_TAC[term_welltyped] >>
       imp_res_tac has_type_IMP >>
       ntac 2 (pop_assum mp_tac) >>
-      simp[Once term_cases] >>
+      simp[] >>
       rw[] >>
       imp_res_tac WELLTYPED_LEMMA >>
       rw[] ) >>
     `∀asl c. R asl c ⇒ C asl c` by (
       rpt gen_tac >>
       simp(List.map Abbr [`B`,`C`,`P`,`Q`,`R`]) >>
+      simp[defthm_def] >>
+      rw[] >- (
+        `safe_def_names defs (Typedef tyname t a r)` by (
+          simp[safe_def_names_def] ) >>
+        res_tac >>
+        map_every qexists_tac[`h1`,`c1'`] >>
+        fs[EVERY_MEM,EVERY2_EVERY] >>
+        rfs[MEM_ZIP,GSYM LEFT_FORALL_IMP_THM] >>
+        METIS_TAC[term_type_cons]) >>
       rw[] >>
       qho_match_abbrev_tac`∃e1. term ddefs (t1 === t2) e1 ∧ [] |- e1` >>
       rfs[] >>
@@ -2192,9 +2378,6 @@ val proves_IMP = store_thm("proves_IMP",
       simp[Abbr`t1`] >>
       simp[Once term_cases] >>
       simp_tac(srw_ss()++boolSimps.DNF_ss)[] >>
-      simp[Once CONJ_COMM] >>
-      simp[Once term_cases] >>
-      simp_tac(srw_ss()++boolSimps.DNF_ss)[] >>
       imp_res_tac holSyntaxTheory.WELLTYPED_LEMMA >>
       simp[] >>
       qpat_assum`term defs X c1`mp_tac >>
@@ -2202,14 +2385,15 @@ val proves_IMP = store_thm("proves_IMP",
       rw[] >>
       `∃ty1. x1 has_type ty1 ∧ type defs (Fun (typeof y) Bool) ty1` by METIS_TAC[has_type_IMP] >>
       pop_assum mp_tac >>
-      simp[Once term_cases] >> rw[] >>
-      pop_assum mp_tac >>
-      simp[Once term_cases] >> rw[] >>
+      simp[] >> rw[] >>
+      qmatch_assum_rename_tac`type defs (typeof y) ty1`[] >>
       CONV_TAC (RESORT_EXISTS_CONV List.rev) >>
-      qexists_tac`tx1` >>
+      qexists_tac`ty1` >>
+      qexists_tac`x1` >>
       simp[RIGHT_EXISTS_AND_THM] >>
       `safe_def_names defs (Typedef tyname t a r)` by (
         simp[safe_def_names_def] ) >>
+      conj_asm1_tac >- METIS_TAC[term_type_cons] >>
       conj_asm1_tac >- METIS_TAC[term_type_cons] >>
       qmatch_assum_abbrev_tac`Abbrev (t2 = t3 === t4)` >>
       `t3 === t4 has_type Bool` by (
@@ -2238,51 +2422,41 @@ val proves_IMP = store_thm("proves_IMP",
       simp_tac(srw_ss()++boolSimps.DNF_ss)[] >>
       simp[Once type_def_def] >>
       `term (Typedef tyname t a r::defs) t x1` by METIS_TAC[term_type_cons] >>
-      qexists_tac`x1`>>simp[] >>
-      simp[Q.SPEC`Var X Y`(CONJUNCT2 (SPEC_ALL term_cases))] >>
-      simp_tac(srw_ss()++boolSimps.DNF_ss)[] >>
+      CONV_TAC SWAP_EXISTS_CONV >> qexists_tac`x1`>>simp[] >>
       simp[Q.SPEC`Comb X Y`(CONJUNCT2 (SPEC_ALL term_cases))] >>
       simp_tac(srw_ss()++boolSimps.DNF_ss)[] >>
+      qexists_tac`ty1`>>simp[] >>
       qexists_tac`x1`>>simp[] >>
-      qexists_tac`tx1`>>simp[] >>
-      qexists_tac`x1`>>simp[] >>
-      simp[Q.SPEC`Const X Y`(CONJUNCT2 (SPEC_ALL term_cases))] >>
-      `a ≠ "@"` by fs[consts_def] >>
-      simp[Once type_def_def] >>
-      simp[Once const_def_def] >>
-      simp[Once const_def_def] >>
-      simp[Once const_def_def] >>
-      simp_tac(srw_ss()++boolSimps.DNF_ss)[] >>
-      simp[Q.SPEC`Fun X Y`(CONJUNCT1 (SPEC_ALL term_cases))] >>
-      simp_tac(srw_ss()++boolSimps.DNF_ss)[] >>
-      simp[Q.SPEC`Var X Y`(CONJUNCT2 (SPEC_ALL term_cases))] >>
-      simp_tac(srw_ss()++boolSimps.DNF_ss)[] >>
-      CONV_TAC SWAP_EXISTS_CONV >> qexists_tac`tx1`>>simp[] >>
-      CONV_TAC SWAP_EXISTS_CONV >> qexists_tac`x1`>>simp[] >>
-      CONV_TAC SWAP_EXISTS_CONV >> qexists_tac`tx1`>>simp[] >>
-      simp[Q.SPEC`Tyapp X Y`(CONJUNCT1 (SPEC_ALL term_cases))] >>
-      simp_tac(srw_ss()++boolSimps.DNF_ss)[] >>
-      simp[Once type_def_def] >>
-      CONV_TAC SWAP_EXISTS_CONV >> qexists_tac`tx1`>>simp[] >>
-      CONV_TAC SWAP_EXISTS_CONV >> qexists_tac`x1`>>simp[] >>
-      qexists_tac`MAP Tyvar (STRING_SORT (tvars x1))` >>
+      CONV_TAC SWAP_EXISTS_CONV >> qexists_tac`ty1`>>simp[] >>
+      qexists_tac`MAP Tyvar (STRING_SORT (tvars t))` >>
       simp[RIGHT_EXISTS_AND_THM] >>
       conj_asm1_tac >- (
         simp[EVERY2_MAP] >>
-        simp[Once term_cases] >>
-        imp_res_tac tvars_IMP >>
-        simp[] >>
-        match_mp_tac EVERY2_refl >>
-        simp[] ) >>
-      fs[safe_def_names_def] >>
-      conj_tac >- METIS_TAC[MEM_Typedef_MEM_consts,consts_def,MEM_MAP,MEM_APPEND] >>
+        simp[EVERY2_refl] ) >>
+      conj_tac >- (
+        METIS_TAC[MEM_Typedef_MEM_consts,consts_def,MEM_MAP,MEM_APPEND] ) >>
+      `a ≠ "@"` by fs[consts_def] >>
+      simp[Q.SPEC`Const X Y`(CONJUNCT2 (SPEC_ALL term_cases))] >>
+      simp[Once type_def_def] >>
+      simp[Once const_def_def] >>
+      simp[Once const_def_def] >>
+      simp[Once const_def_def] >>
+      simp_tac(srw_ss()++boolSimps.DNF_ss)[] >>
+      qexists_tac`x1`>>simp[]>>
+      qexists_tac`ty1`>>simp[]>>
+      qexists_tac`ty1`>>simp[]>>
+      simp[Once term_cases] >>
+      simp_tac(srw_ss()++boolSimps.DNF_ss)[] >>
+      simp[Once type_def_def] >>
+      qexists_tac`x1`>>simp[]>>
       HINT_EXISTS_TAC >> simp[] >>
       conj_tac >- METIS_TAC[MEM_Typedef_MEM_consts,consts_def,MEM_MAP,MEM_APPEND] >>
-      match_mp_tac(List.nth(CONJUNCTS proves_rules,27)) >>
+      match_mp_tac(List.nth(CONJUNCTS proves_rules,28)) >>
       imp_res_tac CLOSED_IMP >>
       simp[] >>
       qexists_tac`y1` >>
       imp_res_tac WELLTYPED_LEMMA >>
+      imp_res_tac tvars_IMP >>
       simp[]) >>
     qsuff_tac`B` >- METIS_TAC[] >>
     simp[Abbr`B`] >>
@@ -2301,7 +2475,7 @@ val proves_IMP = store_thm("proves_IMP",
         simp[Once holSyntaxTheory.proves_cases] >>
         rpt disj2_tac >>
         qexists_tac`[]` >> simp[] >>
-        match_mp_tac (List.nth(CONJUNCTS holSyntaxTheory.proves_rules,25)) >>
+        match_mp_tac (List.nth(CONJUNCTS holSyntaxTheory.proves_rules,26)) >>
         simp[] >> PROVE_TAC[] ) >>
       qexists_tac`x1` >>
       conj_tac >- (
@@ -2333,7 +2507,7 @@ val proves_IMP = store_thm("proves_IMP",
         rpt disj2_tac >>
         qexists_tac`[]` >> simp[] >>
         simp[Abbr`ddefs`] >>
-        match_mp_tac (List.nth(CONJUNCTS holSyntaxTheory.proves_rules,25)) >>
+        match_mp_tac (List.nth(CONJUNCTS holSyntaxTheory.proves_rules,26)) >>
         simp[] >>
         qexists_tac`x` >>
         HINT_EXISTS_TAC >>
@@ -2390,7 +2564,7 @@ val proves_IMP = store_thm("proves_IMP",
         rpt disj2_tac >>
         qexists_tac`[]` >> simp[] >>
         simp[Abbr`ddefs`] >>
-        match_mp_tac (List.nth(CONJUNCTS holSyntaxTheory.proves_rules,25)) >>
+        match_mp_tac (List.nth(CONJUNCTS holSyntaxTheory.proves_rules,26)) >>
         simp[] >>
         qexists_tac`x` >>
         HINT_EXISTS_TAC >>
@@ -2439,13 +2613,13 @@ val proves_IMP = store_thm("proves_IMP",
       simp[Once holSyntaxTheory.proves_cases] >>
       rpt disj2_tac >>
       qexists_tac`[]` >> simp[] >>
-      match_mp_tac (List.nth(CONJUNCTS holSyntaxTheory.proves_rules,25)) >>
+      match_mp_tac (List.nth(CONJUNCTS holSyntaxTheory.proves_rules,26)) >>
       simp[] >>
       qexists_tac`ARB` >>
       HINT_EXISTS_TAC >>
       HINT_EXISTS_TAC >>
       simp[] >> disj1_tac >>
-      match_mp_tac (List.nth(CONJUNCTS holSyntaxTheory.proves_rules,13)) >>
+      match_mp_tac (List.nth(CONJUNCTS holSyntaxTheory.proves_rules,14)) >>
       METIS_TAC[] ) >>
     res_tac >>
     qexists_tac`t1` >>
@@ -2460,30 +2634,16 @@ val proves_IMP = store_thm("proves_IMP",
     simp[Abbr`l`,Abbr`r`] >>
     disch_then kall_tac >>
     srw_tac[boolSimps.DNF_ss][] >>
-    simp[Once term_cases] >>
-    srw_tac[boolSimps.DNF_ss][] >>
-    CONV_TAC SWAP_EXISTS_CONV >>
     qexists_tac`ty1` >> simp[] >>
     simp[Once term_cases] >>
     srw_tac[boolSimps.DNF_ss][] >>
-    simp[Once term_cases] >>
-    srw_tac[boolSimps.DNF_ss][] >>
-    simp[Once term_cases] >>
-    srw_tac[boolSimps.DNF_ss][] >>
-    CONV_TAC (RESORT_EXISTS_CONV List.rev) >>
-    qexists_tac`ty1'` >>
     qexists_tac`ty1` >> simp[] >>
-    simp[Once term_cases] >>
-    srw_tac[boolSimps.DNF_ss][] >>
-    CONV_TAC SWAP_EXISTS_CONV >>
+    qexists_tac`ty1'` >> simp[] >>
     qexists_tac`ty1` >> simp[] >>
-    simp[Once term_cases] >>
-    srw_tac[boolSimps.DNF_ss][] >>
-    simp[Once term_cases] >>
-    srw_tac[boolSimps.DNF_ss][] >>
-    qexists_tac`ty1`>>simp[]>>
-    qexists_tac`ty1'` >> simp[Abbr`P`] >>
-    match_mp_tac(List.nth(CONJUNCTS proves_rules,28)) >>
+    qexists_tac`ty1` >> simp[] >>
+    qexists_tac`ty1'` >> simp[] >>
+    simp[Abbr`P`] >>
+    match_mp_tac(List.nth(CONJUNCTS proves_rules,29)) >>
     rw[] ) >>
   conj_tac >- (
     rw[seq_trans_def] >>
@@ -2498,10 +2658,6 @@ val proves_IMP = store_thm("proves_IMP",
     srw_tac[boolSimps.DNF_ss][] >>
     rw[Once term_cases] >>
     srw_tac[boolSimps.DNF_ss][] >>
-    rw[Once term_cases] >>
-    srw_tac[boolSimps.DNF_ss][] >>
-    rw[Once term_cases] >>
-    srw_tac[boolSimps.DNF_ss][] >>
     fs[holSyntaxTheory.WELLTYPED] >>
     imp_res_tac holSyntaxTheory.WELLTYPED_LEMMA >>
     fs[] >> rw[] >>
@@ -2509,59 +2665,60 @@ val proves_IMP = store_thm("proves_IMP",
     simp[] >>
     disch_then(qspecl_then[`defs`,`x1`]mp_tac) >>
     simp[] >>
-    simp[Once term_cases] >>
     srw_tac[boolSimps.DNF_ss][] >>
     qexists_tac`x1` >>
-    qexists_tac`tx1` >>
-    qexists_tac`tx1` >>
+    HINT_EXISTS_TAC >>
+    HINT_EXISTS_TAC >>
     rw[] >>
-    simp[Once term_cases] >>
-    match_mp_tac(List.nth(CONJUNCTS proves_rules,29)) >>
-    qexists_tac`y1` >> rw[] >>
-    qpat_assum`type Y Bool Z`mp_tac >>
-    simp[Once term_cases] >> rw[] >>
-    rw[]) >>
+    match_mp_tac(List.nth(CONJUNCTS proves_rules,30)) >>
+    qexists_tac`y1` >> rw[]) >>
   rpt gen_tac >> strip_tac >>
   simp[seq_trans_def] >>
+  conj_tac >- fs[seq_trans_def] >>
   simp[Once term_cases,PULL_EXISTS] >>
   exists_tac(EX_def|>Q.SPECL[`x`,`Fun Ind Ind`,`b`]|>concl|>rhs|>rator|>rand) >>
   simp[Once term_cases] >>
-  fs[good_defs_def] >>
   qspecl_then[`defs`,`"?"`]imp_res_tac MEM_Constdef_const_def >>
-  simp[] >>
-  ntac 9 (simp[Once term_cases]) >>
-  simp[Once term_cases,PULL_EXISTS] >>
+  fs[find_index_def] >> rw[] >>
+  pop_assum mp_tac >>
+  discharge_hyps >- fs[good_defs_def] >> strip_tac >>
+  simp[Once term_cases] >>
   qspecl_then[`defs`,`"!"`]imp_res_tac MEM_Constdef_const_def >>
-  simp[Once(Q.SPEC`Const X Y`(CONJUNCT2 (SPEC_ALL term_cases))),PULL_EXISTS] >>
+  fs[find_index_def] >> rw[] >>
+  pop_assum mp_tac >>
+  discharge_hyps >- fs[good_defs_def] >> strip_tac >>
   simp[Once FA_def] >>
-  ntac 7 (simp[Once term_cases]) >>
+  simp[Once term_cases] >>
+  simp[Once(Q.SPEC`Const X Y`(CONJUNCT2 (SPEC_ALL term_cases))),PULL_EXISTS] >>
   Q.PAT_ABBREV_TAC`p1 = holSyntax$Var XX (Fun Z Bool)` >>
   Q.PAT_ABBREV_TAC`p2 = Var XX (Fun Z Bool)` >>
   Q.PAT_ABBREV_TAC`q1 = holSyntax$Abs  X Y Z` >>
   Q.PAT_ABBREV_TAC`q2 = Abs  X Y Z` >>
   qspecl_then[`p1`,`q1`,`p2===q2`]mp_tac term_equation >>
   discharge_hyps >- (
-    simp[Abbr`p1`,Abbr`q1`,holSyntaxTheory.EQUATION_HAS_TYPE_BOOL,good_defs_def] ) >>
+    simp[Abbr`p1`,Abbr`q1`,holSyntaxTheory.EQUATION_HAS_TYPE_BOOL] ) >>
   simp[] >> disch_then kall_tac >>
-  simp[PULL_EXISTS] >>
-  CONV_TAC SWAP_EXISTS_CONV >> qexists_tac`p2` >>
-  CONV_TAC SWAP_EXISTS_CONV >> qexists_tac`q2` >>
+  CONV_TAC SWAP_EXISTS_CONV >> qexists_tac`Ind` >>
+  CONV_TAC SWAP_EXISTS_CONV >> qexists_tac`Ind` >>
   simp[GSYM PULL_EXISTS] >>
   mp_tac term_Truth >>
-  discharge_hyps >- simp[good_defs_def] >> strip_tac >>
+  discharge_hyps >- simp[] >> strip_tac >>
+  simp[GSYM CONJ_ASSOC] >>
+  conj_asm1_tac >- ( simp[Abbr`p1`,Abbr`p2`] ) >>
+  conj_asm1_tac >- ( simp[Abbr`q1`,Abbr`q2`] ) >>
   conj_asm1_tac >- (
-    unabbrev_all_tac >>
-    simp[Once term_cases] >>
-    simp[Once term_cases] >>
-    simp[Once term_cases] >>
-    simp[Once term_cases] >>
-    simp[Once term_cases] >>
-    simp[Once term_cases] ) >>
-  simp[Once term_cases] >>
-  simp[Once term_cases] >>
-  conj_tac >- (
+    match_mp_tac term_equation_matchable >>
+    simp[typeof_shadow_def] >>
+    simp[holSyntaxTheory.EQUATION_HAS_TYPE_BOOL,welltyped_equation] >>
+    simp[Abbr`p1`,Abbr`q1`] >>
+    conj_tac >- (
+      unabbrev_all_tac >>
+      simp[holSyntaxTheory.equation_def,equation_def] ) >>
+    match_mp_tac term_equation_matchable >>
+    simp[Abbr`q2`,holSyntaxTheory.EQUATION_HAS_TYPE_BOOL] ) >>
+  conj_asm1_tac >- (
     match_mp_tac term_Implies >>
-    simp[good_defs_def] >>
+    simp[] >>
     simp[Once holSyntaxTheory.has_type_cases] >>
     simp[Once holSyntaxTheory.has_type_cases] >>
     simp[Once holSyntaxTheory.has_type_cases] >>
@@ -2573,225 +2730,135 @@ val proves_IMP = store_thm("proves_IMP",
     simp[Once holSyntaxTheory.has_type_cases] >>
     simp[Once holSyntaxTheory.has_type_cases] >>
     simp[Once holSyntaxTheory.has_type_cases] >>
-    conj_tac >- (
-      match_mp_tac (GEN_ALL term_Forall) >>
-      simp[good_defs_def] >>
-      simp[Once term_cases] >>
-      simp[Once term_cases] >>
-      simp[Once holSyntaxTheory.has_type_cases] >>
-      simp[Once holSyntaxTheory.has_type_cases] >>
-      simp[Once holSyntaxTheory.has_type_cases] >>
-      simp[Once holSyntaxTheory.has_type_cases] >>
-      simp[Once holSyntaxTheory.has_type_cases] >>
-      simp[Once holSyntaxTheory.has_type_cases] >>
-      simp[Once holSyntaxTheory.has_type_cases] >>
-      reverse conj_tac >- simp[Once term_cases] >>
-      match_mp_tac term_Implies >>
-      simp[good_defs_def] >>
-      simp[Once holSyntaxTheory.has_type_cases] >>
-      simp[Once holSyntaxTheory.has_type_cases] >>
-      simp[Once holSyntaxTheory.has_type_cases] >>
-      simp[Once holSyntaxTheory.has_type_cases] >>
-      simp[Once term_cases] >>
-      simp[Once term_cases] >>
-      simp[Once term_cases] >>
-      simp[Once term_cases] >>
-      simp[Once term_cases] ) >>
-    simp[Once term_cases] >>
+    match_mp_tac (GEN_ALL term_Forall) >>
+    simp[] >>
+    simp[Once holSyntaxTheory.has_type_cases] >>
+    simp[Once holSyntaxTheory.has_type_cases] >>
+    simp[Once holSyntaxTheory.has_type_cases] >>
+    simp[Once holSyntaxTheory.has_type_cases] >>
+    simp[Once holSyntaxTheory.has_type_cases] >>
+    simp[Once holSyntaxTheory.has_type_cases] >>
+    simp[Once holSyntaxTheory.has_type_cases] >>
+    match_mp_tac term_Implies >>
+    simp[] >>
+    simp[Once holSyntaxTheory.has_type_cases] >>
+    simp[Once holSyntaxTheory.has_type_cases] >>
+    simp[Once holSyntaxTheory.has_type_cases] >>
+    simp[Once holSyntaxTheory.has_type_cases] >>
     simp[Once term_cases] ) >>
-  simp[Once term_cases,PULL_EXISTS] >>
-  qexists_tac`Fun Ind Ind` >>
+  conj_tac >- (
+    match_mp_tac term_equation_matchable >>
+    simp[typeof_shadow_def,Once FA_def,holSyntaxTheory.EQUATION_HAS_TYPE_BOOL,Abbr`p1`] >>
+    match_mp_tac (GEN_ALL term_Forall) >>
+    simp[] >>
+    rpt(simp[Once holSyntaxTheory.has_type_cases])) >>
   simp[Once term_cases] >>
   simp[Once term_cases] >>
   qexists_tac`AN (O1 Ind Ind (Var "f" (Fun Ind Ind))) (NO (OT Ind Ind (Var "f" (Fun Ind Ind))))` >>
   conj_tac >- (
     match_mp_tac term_And >>
-    simp[good_defs_def] >>
-    simp[Once holSyntaxTheory.has_type_cases] >>
-    simp[Once holSyntaxTheory.has_type_cases] >>
-    simp[Once holSyntaxTheory.has_type_cases] >>
-    simp[Once holSyntaxTheory.has_type_cases] >>
-    simp[Once holSyntaxTheory.has_type_cases] >>
-    simp[Once holSyntaxTheory.has_type_cases] >>
-    simp[Once holSyntaxTheory.has_type_cases] >>
-    simp[Once holSyntaxTheory.has_type_cases] >>
+    simp[] >>
+    ntac 8 (simp[Once holSyntaxTheory.has_type_cases]) >>
     conj_tac >- (
-      simp[Once term_cases] >>
       simp[Once term_cases,O1_def] >>
-      simp[Once term_cases] >>
-      simp[Once term_cases] >>
-      simp[Once term_cases] >>
-      simp[Once term_cases] >>
       qspecl_then[`defs`,`"ONE_ONE"`]imp_res_tac MEM_Constdef_const_def >>
+      fs[find_index_def] >>
+      reverse conj_tac >- simp[Once term_cases] >> rw[] >>
+      pop_assum mp_tac >>
+      discharge_hyps >- fs[good_defs_def] >> strip_tac >>
       simp[Once term_cases] >>
       simp[Once term_cases] >>
-      simp[Once term_cases] >>
-      simp[Once term_cases] >>
-      reverse conj_tac >- (
-        simp[Once term_cases] >>
-        simp[Once term_cases] >>
-        simp[Once term_cases] ) >>
-      match_mp_tac (GEN_ALL term_Forall) >>
-      simp[good_defs_def] >>
-      simp[Once term_cases] >>
-      simp[Once term_cases] >>
-      simp[Once holSyntaxTheory.has_type_cases] >>
-      simp[Once holSyntaxTheory.has_type_cases] >>
-      simp[Once holSyntaxTheory.has_type_cases] >>
-      simp[Once holSyntaxTheory.has_type_cases] >>
-      simp[Once holSyntaxTheory.has_type_cases] >>
-      simp[Once holSyntaxTheory.has_type_cases] >>
-      simp[holSyntaxTheory.EQUATION_HAS_TYPE_BOOL] >>
-      conj_tac >- (
+      conj_asm1_tac >- (
         match_mp_tac (GEN_ALL term_Forall) >>
-        simp[good_defs_def] >>
-        simp[Once term_cases] >>
-        simp[Once term_cases] >>
+        simp[Once holSyntaxTheory.has_type_cases] >>
+        simp[Once holSyntaxTheory.has_type_cases] >>
+        simp[Once holSyntaxTheory.has_type_cases] >>
         simp[Once holSyntaxTheory.has_type_cases] >>
         simp[Once holSyntaxTheory.has_type_cases] >>
         simp[Once holSyntaxTheory.has_type_cases] >>
         simp[holSyntaxTheory.EQUATION_HAS_TYPE_BOOL] >>
+        match_mp_tac (GEN_ALL term_Forall) >>
+        simp[Once holSyntaxTheory.has_type_cases] >>
+        simp[Once holSyntaxTheory.has_type_cases] >>
+        simp[Once holSyntaxTheory.has_type_cases] >>
+        simp[holSyntaxTheory.EQUATION_HAS_TYPE_BOOL] >>
+        match_mp_tac term_Implies >>
+        simp[holSyntaxTheory.EQUATION_HAS_TYPE_BOOL] >>
         conj_tac >- (
-          match_mp_tac term_Implies >>
-          simp[good_defs_def] >>
+          match_mp_tac term_equation_matchable >>
           simp[holSyntaxTheory.EQUATION_HAS_TYPE_BOOL] >>
-          conj_tac >- (
-            match_mp_tac (MP_CANON(DISCH_ALL(snd(EQ_IMP_RULE(UNDISCH (SPEC_ALL term_equation)))))) >>
-            simp[holSyntaxTheory.EQUATION_HAS_TYPE_BOOL,good_defs_def] >>
-            Q.PAT_ABBREV_TAC`l1 = Comb X Y` >>
-            Q.PAT_ABBREV_TAC`r1 = Comb X Y` >>
-            map_every qexists_tac[`l1`,`r1`] >>
-            simp[Abbr`l1`,Abbr`r1`] >>
-            simp[Once term_cases] >>
-            simp[Once term_cases] >>
-            simp[Once term_cases] >>
-            simp[Once term_cases] >>
-            simp[Once term_cases] >>
-            simp[Once term_cases] >>
-            simp[Once term_cases] >>
-            simp[Once term_cases] >>
-            simp[Once term_cases] >>
-            simp[Once term_cases] >>
-            simp[Once term_cases] >>
-            simp[Once term_cases] >>
-            simp[Once term_cases] >>
-            simp[Once term_cases] ) >>
-          match_mp_tac (MP_CANON(DISCH_ALL(snd(EQ_IMP_RULE(UNDISCH (SPEC_ALL term_equation)))))) >>
-          simp[holSyntaxTheory.EQUATION_HAS_TYPE_BOOL,good_defs_def] >>
-          Q.PAT_ABBREV_TAC`l1 = Var X Y` >>
-          Q.PAT_ABBREV_TAC`r1 = Var X Y` >>
-          map_every qexists_tac[`l1`,`r1`] >>
-          simp[Abbr`l1`,Abbr`r1`] >>
-          simp[Once term_cases] >>
-          simp[Once term_cases] >>
           simp[Once term_cases] >>
           simp[Once term_cases] ) >>
-        simp[Once term_cases] ) >>
-      simp[Once term_cases] ) >>
+        match_mp_tac term_equation_matchable >>
+        simp[holSyntaxTheory.EQUATION_HAS_TYPE_BOOL] ) >>
+      match_mp_tac term_equation_matchable >>
+      simp[typeof_shadow_def,Once FA_def] >>
+      simp[holSyntaxTheory.EQUATION_HAS_TYPE_BOOL,welltyped_equation] >>
+      simp[holSyntaxTheory.equation_def] ) >>
     simp[Once term_cases,NO_def] >>
     qspecl_then[`defs`,`"~"`]imp_res_tac MEM_Constdef_const_def >>
-    simp[Once term_cases] >>
-    simp[Once term_cases] >>
-    simp[Once term_cases] >>
-    simp[Once term_cases] >>
-    simp[Once term_cases] >>
-    conj_tac >- (
+    fs[find_index_def] >> rpt(qpat_assum`T`kall_tac) >>
+    pop_assum mp_tac >>
+    discharge_hyps >- fs[good_defs_def] >> strip_tac >>
+    simp[Once term_cases,GSYM CONJ_ASSOC] >>
+    conj_asm1_tac >- (
       match_mp_tac term_Implies >>
-      simp[good_defs_def] >>
+      simp[] >>
       simp[Once holSyntaxTheory.has_type_cases] >>
       simp[Once holSyntaxTheory.has_type_cases] >>
-      simp[Once term_cases] >>
-      simp[Once term_cases] >>
       qspecl_then[`defs`,`"F"`]imp_res_tac MEM_Constdef_const_def >>
+      fs[find_index_def] >> rpt(qpat_assum`T`kall_tac) >>
+      pop_assum mp_tac >> discharge_hyps >- fs[good_defs_def] >> strip_tac >>
       simp[Once term_cases,FF_def] >>
-      simp[Once term_cases] >>
-      match_mp_tac(GEN_ALL term_Forall) >>
-      simp[good_defs_def] >>
-      simp[Once term_cases] >>
-      simp[Once term_cases] >>
-      simp[Once term_cases] >>
-      simp[Once term_cases] >>
+      conj_tac >- (
+        match_mp_tac(GEN_ALL term_Forall) >>
+        simp[Once holSyntaxTheory.has_type_cases] ) >>
+      match_mp_tac term_equation_matchable >>
+      simp[typeof_shadow_def,Once FA_def] >>
+      simp[holSyntaxTheory.EQUATION_HAS_TYPE_BOOL] >>
+      match_mp_tac (GEN_ALL term_Forall) >>
       simp[Once holSyntaxTheory.has_type_cases] ) >>
+    conj_asm1_tac >- (
+      match_mp_tac term_equation_matchable >>
+      simp[typeof_shadow_def,holSyntaxTheory.EQUATION_HAS_TYPE_BOOL] >>
+      simp[IM_def] ) >>
     simp[Once term_cases,OT_def] >>
     qspecl_then[`defs`,`"ONTO"`]imp_res_tac MEM_Constdef_const_def >>
-    simp[Once term_cases] >>
-    simp[Once term_cases] >>
-    simp[Once term_cases] >>
-    simp[Once term_cases] >>
-    simp[Once term_cases] >>
-    simp[Once term_cases] >>
-    simp[Once term_cases] >>
-    simp[Once term_cases] >>
-    simp[Once term_cases] >>
-    conj_tac >- (
+    fs[find_index_def] >> rpt(qpat_assum`T`kall_tac) >>
+    pop_assum mp_tac >> discharge_hyps >- fs[good_defs_def] >> strip_tac >>
+    simp[Once term_cases,GSYM CONJ_ASSOC] >>
+    conj_asm1_tac >- simp[Once term_cases] >>
+    conj_asm1_tac >- (
       match_mp_tac(GEN_ALL term_Forall) >>
-      simp[good_defs_def] >>
-      simp[Once term_cases] >>
-      simp[Once term_cases] >>
       simp[Once holSyntaxTheory.has_type_cases] >>
       simp[Once holSyntaxTheory.has_type_cases] >>
       simp[Once holSyntaxTheory.has_type_cases] >>
       simp[holSyntaxTheory.EQUATION_HAS_TYPE_BOOL] >>
       simp[Once term_cases,EX_def] >>
-      ntac 9 (simp[Once term_cases]) >>
+      simp[Once term_cases] >>
       conj_tac >- (
-        conj_tac >- (
+        conj_asm1_tac >- (
           match_mp_tac (GEN_ALL term_Forall) >>
-          simp[good_defs_def] >>
-          simp[Once term_cases] >>
-          simp[Once term_cases] >>
           ntac 6 ( simp[Once holSyntaxTheory.has_type_cases] )>>
           simp[Once holSyntaxTheory.has_type_cases,Abbr`p1`] >>
-          simp[Once holSyntaxTheory.has_type_cases] >>
-          simp[Once holSyntaxTheory.has_type_cases] >>
-          simp[Once holSyntaxTheory.has_type_cases] >>
-          simp[Once holSyntaxTheory.has_type_cases] >>
-          simp[Once holSyntaxTheory.has_type_cases] >>
-          simp[Once holSyntaxTheory.has_type_cases] >>
-          reverse conj_tac >- simp[Once term_cases] >>
-          match_mp_tac term_Implies >>
-          simp[good_defs_def] >>
-          ntac 12 ( simp[Once holSyntaxTheory.has_type_cases] ) >>
-          reverse conj_tac >- (
-            ntac 2 (simp[Once term_cases])) >>
-          match_mp_tac (GEN_ALL term_Forall) >>
-          simp[good_defs_def] >>
-          simp[Once term_cases] >>
-          simp[Once term_cases] >>
-          ntac 7 ( simp[Once holSyntaxTheory.has_type_cases] )>>
-          reverse conj_tac >- simp[Once term_cases] >>
-          match_mp_tac term_Implies >>
-          simp[good_defs_def] >>
-          ntac 4 ( simp[Once holSyntaxTheory.has_type_cases] )>>
-          ntac 5 (simp[Once term_cases])) >>
-        simp[Once term_cases] >>
-        simp[Once term_cases] >>
-        reverse conj_tac >- (
-          Q.PAT_ABBREV_TAC`eq:holSyntax$term = a === b` >>
-          qsuff_tac`eq has_type Bool` >- PROVE_TAC[holSyntaxTheory.WELLTYPED,holSyntaxTheory.WELLTYPED_LEMMA] >>
-          simp[holSyntaxTheory.EQUATION_HAS_TYPE_BOOL,Abbr`eq`] ) >>
-        match_mp_tac (MP_CANON(DISCH_ALL(snd(EQ_IMP_RULE(UNDISCH (SPEC_ALL term_equation)))))) >>
-        simp[holSyntaxTheory.EQUATION_HAS_TYPE_BOOL] >>
-        simp[good_defs_def] >>
-        Q.PAT_ABBREV_TAC`l1 = Var X Y` >>
-        Q.PAT_ABBREV_TAC`r1 = Comb X Y` >>
-        map_every qexists_tac[`l1`,`r1`] >>
-        simp[Abbr`l1`,Abbr`r1`] >>
-        simp[Once term_cases] >>
-        simp[Once term_cases] >>
-        simp[Once term_cases] >>
-        simp[Once term_cases] >>
-        simp[Once term_cases] >>
-        simp[Once term_cases] >>
-        simp[Once term_cases] >>
-        simp[Once term_cases] >>
-        simp[Once term_cases] ) >>
+          rpt (simp[Once holSyntaxTheory.has_type_cases])) >>
+        match_mp_tac term_equation_matchable >>
+        simp[typeof_shadow_def,holSyntaxTheory.EQUATION_HAS_TYPE_BOOL,Abbr`p1`] >>
+        simp[Once FA_def] ) >>
+      simp[welltyped_equation] >>
+      reverse conj_tac >- (
+        Q.PAT_ABBREV_TAC`eq:holSyntax$term = a === b` >>
+        qsuff_tac`eq has_type Bool` >- PROVE_TAC[holSyntaxTheory.WELLTYPED,holSyntaxTheory.WELLTYPED_LEMMA] >>
+        simp[holSyntaxTheory.EQUATION_HAS_TYPE_BOOL,Abbr`eq`] ) >>
+      match_mp_tac term_equation_matchable >>
+      simp[holSyntaxTheory.EQUATION_HAS_TYPE_BOOL] >>
       simp[Once term_cases] ) >>
-    simp[Once term_cases] >>
-    simp[Once term_cases] >>
-    simp[Once term_cases] ) >>
+    simp[typeof_shadow_def] >>
+    match_mp_tac term_equation_matchable >>
+    simp[holSyntaxTheory.EQUATION_HAS_TYPE_BOOL,Once FA_def,welltyped_equation] >>
+    simp[holSyntaxTheory.equation_def] ) >>
   simp[GSYM EX_def,Abbr`p2`] >>
-  ACCEPT_TAC(List.nth(CONJUNCTS proves_rules,30)))
+  ACCEPT_TAC(List.nth(CONJUNCTS proves_rules,31)))
 
 val soundness = store_thm("soundness",
   ``is_model M ⇒ ∀dh t. dh |- t ⇒ hol_seq (dh,t)``,
@@ -2857,12 +2924,15 @@ val proves_cons_def = store_thm("proves_cons_def",
   ``is_model M ⇒ ∀defs h c d. (defs,h) |- c ⇒ context_ok (d::defs) ⇒ (d::defs,h) |- c``,
   rw[] >>
   Cases_on`d` >- (
-    match_mp_tac(List.nth(CONJUNCTS holSyntaxTheory.proves_rules,23)) >>
+    match_mp_tac(List.nth(CONJUNCTS holSyntaxTheory.proves_rules,24)) >>
     imp_res_tac proves_IMP >>
     fs[def_ok_def,deftm_def,pred_setTheory.SUBSET_DEF,good_defs_def,defcnds_ok_def] >>
     imp_res_tac term_ok_welltyped >>
-    fs[consts_def,ALL_DISTINCT_APPEND,consts_aux_def] ) >>
-  match_mp_tac(List.nth(CONJUNCTS holSyntaxTheory.proves_rules,25)) >>
+    fs[consts_def,ALL_DISTINCT_APPEND,consts_aux_def] >>
+    fs[MAP_MAP_o,combinTheory.o_DEF,UNCURRY,ETA_AX] >>
+    simp[MEM_MAP,EXISTS_PROD] >>
+    METIS_TAC[]) >>
+  match_mp_tac(List.nth(CONJUNCTS holSyntaxTheory.proves_rules,26)) >>
   simp[] >>
   imp_res_tac proves_IMP >>
   fs[def_ok_def,deftm_def,good_defs_def,defcnds_ok_def] >>
